# Saved by TopBraid on Wed Aug 04 18:33:52 CEST 2010
# baseURI: http://purl.org/ontology/pbo/core#
# imports: http://purl.org/ontology/olo/core
# imports: http://purl.org/NET/c4dm/event.owl
# imports: http://purl.org/ontology/bibo/
# imports: http://purl.org/dc/elements/1.1/
# imports: http://www.w3.org/2003/06/sw-vocab-status/ns
# imports: http://purl.org/ontology/co/core
# imports: http://purl.org/vocab/frbr/core

@prefix bibo:    <http://purl.org/ontology/bibo/> .
@prefix co:      <http://purl.org/ontology/co/core#> .
@prefix dc:      <http://purl.org/dc/elements/1.1/> .
@prefix dcterms:  <http://purl.org/dc/terms/> .
@prefix frbr:    <http://purl.org/vocab/frbr/core#> .
@prefix olo:     <http://purl.org/ontology/olo/core#> .
@prefix owl:     <http://www.w3.org/2002/07/owl#> .
@prefix pbo:     <http://purl.org/ontology/pbo/core#> .
@prefix rdf:     <http://www.w3.org/1999/02/22-rdf-syntax-ns#> .
@prefix rdfs:    <http://www.w3.org/2000/01/rdf-schema#> .
@prefix time:    <http://www.w3.org/2006/time#> .
@prefix vs:      <http://www.w3.org/2003/06/sw-vocab-status/ns#> .
@prefix xsd:     <http://www.w3.org/2001/XMLSchema#> .

pbo:  rdf:type owl:Ontology ;
      dc:creator <http://foaf.me/zazi#me> ;
      dc:date "2010-08-04T17:33:52+01:00"^^xsd:dateTime ;
      dc:description """The Play Back Ontology specification provides basic concepts and properties 
for describing concepts that are related to the play back domain, e.g. an playlist, play back count and skip counter 
on/ for the Semantic Web. This document contains a RDF description of the Play Back Ontology."""@en ;
      dc:title "The Play Back Ontology"@en ;
      owl:imports <http://purl.org/NET/c4dm/event.owl> , bibo: , <http://purl.org/ontology/olo/core> , <http://www.w3.org/2003/06/sw-vocab-status/ns> , <http://purl.org/vocab/frbr/core> , <http://purl.org/ontology/co/core> , dc: ;
      owl:versionInfo 0.55 .

pbo:FixedPlaylist
      rdf:type owl:Class ;
      rdfs:comment """A (sub) playlist of a fixed length and a fixed order. This concept should be used to express static relations, 
e.g. \"those three music tracks must always be played in a row\"."""@en ;
      rdfs:isDefinedBy pbo: ;
      rdfs:label "Fixed Playlist"@en ;
      rdfs:subClassOf pbo:Playlist ;
      vs:term_status "testing"@en .

pbo:MediaActionCounter
      rdf:type owl:Class ;
      rdfs:comment "A media action counter. Media actions are for example play back or skip events."^^xsd:string ;
      rdfs:isDefinedBy pbo: ;
      rdfs:label "Media Action Counter"@en ;
      rdfs:subClassOf co:Counter ;
      vs:term_status "unstable"@en .

pbo:PlayBackCounter
      rdf:type owl:Class ;
      rdfs:comment "A play back counter, e.g. to count the playback of a media object."^^xsd:string ;
      rdfs:isDefinedBy pbo: ;
      rdfs:label "Play Back Counter"@en ;
      rdfs:subClassOf pbo:MediaActionCounter ;
      vs:term_status "unstable"@en .

pbo:Playlist
      rdf:type owl:Class ;
      rdfs:comment "A playlist of specific media items, e.g. music tracks, videos or slides."@en ;
      rdfs:isDefinedBy pbo: ;
      rdfs:label "Playlist"@en ;
      rdfs:subClassOf olo:OrderedList , bibo:Document ;
      vs:term_status "unstable"@en .

pbo:PlaylistSlot
      rdf:type owl:Class ;
      rdfs:comment """A playlist slot. It could contain e.g. a music track, a video or a slide, and maybe related with some 
additional properties. However, it could maybe also included a \"sub\" playlist, e.g. to keep a fixed sequence of some tracks."""@en ;
      rdfs:isDefinedBy pbo: ;
      rdfs:label "Playlist Slot"@en ;
      rdfs:subClassOf olo:Slot ;
      rdfs:subClassOf
              [ rdf:type owl:Restriction ;
                owl:minCardinality "1"^^xsd:nonNegativeInteger ;
                owl:onProperty pbo:playlist_item
              ] ;
      vs:term_status "testing"@en .

pbo:SkipCounter
      rdf:type owl:Class ;
      rdfs:comment "A skip counter, e.g. to count skip events of a media object."^^xsd:string ;
      rdfs:isDefinedBy pbo: ;
      rdfs:label "Skip Counter"^^xsd:string ;
      rdfs:subClassOf pbo:MediaActionCounter ;
      vs:term_status "unstable"^^xsd:string .

pbo:SkipEvent
      rdf:type owl:Class ;
      rdfs:comment "A specific skip event of something."^^xsd:string ;
      rdfs:isDefinedBy pbo: ;
      rdfs:label "Skip Event"^^xsd:string ;
      rdfs:subClassOf co:ScrobbleEvent ;
      vs:term_status "testing"^^xsd:string .

pbo:media_object
      rdf:type owl:ObjectProperty ;
      rdfs:comment "Associates a media object to its related counter."@en ;
      rdfs:domain pbo:MediaActionCounter ;
      rdfs:isDefinedBy pbo: ;
      rdfs:label "has media object"@en ;
      rdfs:range
              [ rdf:type owl:Class ;
                owl:unionOf (bibo:Document frbr:Endeavour)
              ] ;
      rdfs:subPropertyOf co:object ;
      vs:term_status "unstable"@en .

pbo:media_scrobble_object
      rdf:type owl:ObjectProperty ;
      rdfs:comment "A media specific scrobble object, e.g. a music track or a video."@en ;
      rdfs:isDefinedBy pbo: ;
      rdfs:label "has media scrobble object"@en ;
      rdfs:range
              [ rdf:type owl:Class ;
                owl:unionOf (bibo:Document frbr:Endeavour)
              ] ;
      rdfs:subPropertyOf co:scrobble_object ;
      vs:term_status "testing"@en .

pbo:playlist
      rdf:type owl:ObjectProperty ;
      rdfs:comment "Associates a playlist to something."@en ;
      rdfs:domain owl:Thing ;
      rdfs:isDefinedBy pbo: ;
      rdfs:label "has playlist"@en ;
      rdfs:range pbo:Playlist ;
      vs:term_status "testing"@en .

pbo:playlist_item
      rdf:type owl:ObjectProperty ;
      rdfs:comment """A specific playlist item, e.g. a music track, video or slides. The range types of this property must be 
based on bibo:Document or frbr:Endeavour (to keep it somehow media based)."""@en ;
      rdfs:domain pbo:PlaylistSlot ;
      rdfs:isDefinedBy pbo: ;
      rdfs:label "has playlist item"@en ;
      rdfs:range
              [ rdf:type owl:Class ;
                owl:unionOf (bibo:Document frbr:Endeavour)
              ] ;
      rdfs:subPropertyOf olo:item ;
      owl:inverseOf
              [ rdf:type owl:ObjectProperty ;
                rdfs:label "is playlist item of"@en
              ] ;
      vs:term_status "unstable"@en .

pbo:playlist_slot
      rdf:type owl:ObjectProperty ;
      rdfs:comment "A specific slot in a playlist."@en ;
      rdfs:domain pbo:Playlist ;
      rdfs:label "has playlist slot"@en ;
      rdfs:range pbo:PlaylistSlot ;
      rdfs:subPropertyOf olo:slot ;
      vs:term_status "testing"@en .

pbo:skip_time
      rdf:type owl:ObjectProperty ;
      rdfs:comment "The moment, when someone skipped the media object, e.g. an instant of a timeline of an audio signal."^^xsd:string ;
      rdfs:domain pbo:SkipEvent ;
      rdfs:isDefinedBy pbo: ;
      rdfs:label "has skip time"^^xsd:string ;
      rdfs:range time:TemporalEntity ;
      rdfs:subPropertyOf <http://purl.org/NET/c4dm/event.owl#factor> ;
      vs:term_status "testing"^^xsd:string .
