<?xml version="1.0" encoding="utf-8"?>
<rdf:RDF
   xmlns:bibo="http://purl.org/ontology/bibo/"
   xmlns:co="http://purl.org/ontology/co/core#"
   xmlns:dc="http://purl.org/dc/elements/1.1/"
   xmlns:dcterms="http://purl.org/dc/terms/"
   xmlns:frbr="http://purl.org/vocab/frbr/core#"
   xmlns:olo="http://purl.org/ontology/olo/core#"
   xmlns:owl="http://www.w3.org/2002/07/owl#"
   xmlns:pbo="http://purl.org/ontology/pbo/core#"
   xmlns:rdf="http://www.w3.org/1999/02/22-rdf-syntax-ns#"
   xmlns:rdfs="http://www.w3.org/2000/01/rdf-schema#"
   xmlns:vs="http://www.w3.org/2003/06/sw-vocab-status/ns#"
   xmlns:xsd="http://www.w3.org/2001/XMLSchema#"
   xml:base="http://purl.org/ontology/pbo/core#">
  <owl:Ontology rdf:about="http://purl.org/ontology/pbo/core#">
    <dc:creator rdf:resource="http://foaf.me/zazi#me"/>
    <dc:date rdf:datatype="http://www.w3.org/2001/XMLSchema#dateTime">2010-07-20T15:21:52+01:00</dc:date>
    <dc:description xml:lang="en">The Play Back Ontology specification provides basic concepts and properties 
for describing a concepts that are related to the play back domain, e.g. an playlist, play back count and skip counter 
on/ for the Semantic Web. This document contains a RDF description of the Play Back Ontology.</dc:description>
    <dc:title xml:lang="en">The Play Back Ontology</dc:title>
    <owl:imports rdf:resource="http://purl.org/dc/elements/1.1/"/>
    <owl:imports rdf:resource="http://purl.org/ontology/bibo/"/>
    <owl:imports rdf:resource="http://purl.org/ontology/co/core"/>
    <owl:imports rdf:resource="http://purl.org/ontology/olo/core"/>
    <owl:imports rdf:resource="http://purl.org/vocab/frbr/core"/>
    <owl:imports rdf:resource="http://www.w3.org/2003/06/sw-vocab-status/ns"/>
    <owl:versionInfo rdf:datatype="http://www.w3.org/2001/XMLSchema#decimal">0.3</owl:versionInfo>
  </owl:Ontology>
  <owl:Class rdf:about="http://purl.org/ontology/pbo/core#FixedPlaylist">
    <rdfs:comment xml:lang="en">A (sub) playlist of a fixed length and a fixed order. This concept should be used to express static relations, 
e.g. "those three music tracks must always be played in a row".</rdfs:comment>
    <rdfs:isDefinedBy rdf:resource="http://purl.org/ontology/pbo/core#"/>
    <rdfs:label xml:lang="en">Fixed Playlist</rdfs:label>
    <rdfs:subClassOf rdf:resource="http://purl.org/ontology/pbo/core#Playlist"/>
    <vs:term_status xml:lang="en">testing</vs:term_status>
  </owl:Class>
  <owl:Class rdf:about="http://purl.org/ontology/pbo/core#Playlist">
    <rdfs:comment xml:lang="en">A playlist of specific media items, e.g. music tracks, videos or slides.</rdfs:comment>
    <rdfs:isDefinedBy rdf:resource="http://purl.org/ontology/pbo/core#"/>
    <rdfs:label xml:lang="en">Playlist</rdfs:label>
    <rdfs:subClassOf rdf:resource="http://purl.org/ontology/bibo/Document"/>
    <rdfs:subClassOf rdf:resource="http://purl.org/ontology/olo/core#OrderedList"/>
    <vs:term_status xml:lang="en">unstable</vs:term_status>
  </owl:Class>
  <owl:Class rdf:about="http://purl.org/ontology/pbo/core#PlaylistSlot">
    <rdfs:comment xml:lang="en">A playlist slot. It could contain e.g. a music track, a video or a slide, and maybe related with some 
additional properties. However, it could maybe also included a "sub" playlist, e.g. to keep a fixed sequence of some tracks.</rdfs:comment>
    <rdfs:isDefinedBy rdf:resource="http://purl.org/ontology/pbo/core#"/>
    <rdfs:label xml:lang="en">Playlist Slot</rdfs:label>
    <rdfs:subClassOf rdf:resource="http://purl.org/ontology/olo/core#Slot"/>
    <rdfs:subClassOf>
      <owl:Restriction>
        <owl:minCardinality rdf:datatype="http://www.w3.org/2001/XMLSchema#nonNegativeInteger">1</owl:minCardinality>
        <owl:onProperty rdf:resource="http://purl.org/ontology/pbo/core#playlist_item"/>
      </owl:Restriction>
    </rdfs:subClassOf>
    <vs:term_status xml:lang="en">testing</vs:term_status>
  </owl:Class>
  <owl:ObjectProperty rdf:about="http://purl.org/ontology/pbo/core#play_back_counter">
    <rdfs:comment xml:lang="en">Associates a play back counter of a specific object. A play back counter is related to  specific co:ScrobbleEvent 
instances, which are the related play back events of an object.</rdfs:comment>
    <rdfs:isDefinedBy rdf:resource="http://purl.org/ontology/pbo/core#"/>
    <rdfs:label xml:lang="en">has play back Counter</rdfs:label>
    <rdfs:subPropertyOf rdf:resource="http://purl.org/ontology/co/core#event_counter"/>
    <vs:term_status xml:lang="en">unstable</vs:term_status>
  </owl:ObjectProperty>
  <owl:ObjectProperty rdf:about="http://purl.org/ontology/pbo/core#play_back_object">
    <rdfs:comment xml:lang="en">Associates a play back object to its related play back counter.</rdfs:comment>
    <rdfs:isDefinedBy rdf:resource="http://purl.org/ontology/pbo/core#"/>
    <rdfs:label xml:lang="en">has play back object</rdfs:label>
    <rdfs:range>
      <rdf:Description>
        <owl:unionOf>
          <rdf:Description>
            <rdf:first rdf:resource="http://purl.org/ontology/bibo/Document"/>
            <rdf:rest>
              <rdf:Description>
                <rdf:first rdf:resource="http://purl.org/vocab/frbr/core#Endeavour"/>
                <rdf:rest rdf:resource="http://www.w3.org/1999/02/22-rdf-syntax-ns#nil"/>
              </rdf:Description>
            </rdf:rest>
          </rdf:Description>
        </owl:unionOf>
      </rdf:Description>
    </rdfs:range>
    <rdfs:subPropertyOf rdf:resource="http://purl.org/ontology/co/core#object"/>
    <vs:term_status xml:lang="en">unstable</vs:term_status>
  </owl:ObjectProperty>
  <owl:ObjectProperty rdf:about="http://purl.org/ontology/pbo/core#playlist">
    <rdf:type rdf:resource="http://www.w3.org/1999/02/22-rdf-syntax-ns#Property"/>
    <rdfs:comment xml:lang="en">Associates a playlist to something.</rdfs:comment>
    <rdfs:domain rdf:resource="http://www.w3.org/2002/07/owl#Thing"/>
    <rdfs:isDefinedBy rdf:resource="http://purl.org/ontology/pbo/core#"/>
    <rdfs:label xml:lang="en">has playlist</rdfs:label>
    <rdfs:range rdf:resource="http://purl.org/ontology/pbo/core#Playlist"/>
    <vs:term_status xml:lang="en">testing</vs:term_status>
  </owl:ObjectProperty>
  <owl:ObjectProperty rdf:about="http://purl.org/ontology/pbo/core#playlist_item">
    <rdfs:comment xml:lang="en">A specific playlist item, e.g. a music track, video or slides. The range types of this property must be 
based on bibo:Document or frbr:Endeavour (to keep it somehow media based).</rdfs:comment>
    <rdfs:domain rdf:resource="http://purl.org/ontology/pbo/core#PlaylistSlot"/>
    <rdfs:isDefinedBy rdf:resource="http://purl.org/ontology/pbo/core#"/>
    <rdfs:label xml:lang="en">has playlist item</rdfs:label>
    <rdfs:range>
      <rdf:Description>
        <owl:unionOf>
          <rdf:Description>
            <rdf:first rdf:resource="http://purl.org/ontology/bibo/Document"/>
            <rdf:rest>
              <rdf:Description>
                <rdf:first rdf:resource="http://purl.org/vocab/frbr/core#Endeavour"/>
                <rdf:rest rdf:resource="http://www.w3.org/1999/02/22-rdf-syntax-ns#nil"/>
              </rdf:Description>
            </rdf:rest>
          </rdf:Description>
        </owl:unionOf>
      </rdf:Description>
    </rdfs:range>
    <rdfs:subPropertyOf rdf:resource="http://purl.org/ontology/olo/core#item"/>
    <owl:inverseOf>
      <owl:ObjectProperty>
        <rdfs:label xml:lang="en">is playlist item of</rdfs:label>
      </owl:ObjectProperty>
    </owl:inverseOf>
    <vs:term_status xml:lang="en">unstable</vs:term_status>
  </owl:ObjectProperty>
  <owl:ObjectProperty rdf:about="http://purl.org/ontology/pbo/core#playlist_slot">
    <rdfs:comment rdf:datatype="http://www.w3.org/2001/XMLSchema#string">A specific slot in a playlist.</rdfs:comment>
    <rdfs:domain rdf:resource="http://purl.org/ontology/pbo/core#Playlist"/>
    <rdfs:label rdf:datatype="http://www.w3.org/2001/XMLSchema#string">has playlist slot</rdfs:label>
    <rdfs:range rdf:resource="http://purl.org/ontology/pbo/core#PlaylistSlot"/>
    <rdfs:subPropertyOf rdf:resource="http://purl.org/ontology/olo/core#slot"/>
    <vs:term_status rdf:datatype="http://www.w3.org/2001/XMLSchema#string">testing</vs:term_status>
  </owl:ObjectProperty>
  <owl:ObjectProperty rdf:about="http://purl.org/ontology/pbo/core#skip_counter">
    <rdfs:comment xml:lang="en">Associates a skip counter of a specific object. A skip counter is related to  specific co:ScrobbleEvent 
instances, which are the related skip events of an object.</rdfs:comment>
    <rdfs:isDefinedBy rdf:resource="http://purl.org/ontology/pbo/core#"/>
    <rdfs:label xml:lang="en">has skip counter</rdfs:label>
    <rdfs:subPropertyOf rdf:resource="http://purl.org/ontology/co/core#event_counter"/>
    <vs:term_status xml:lang="en">unstable</vs:term_status>
  </owl:ObjectProperty>
  <owl:ObjectProperty rdf:about="http://purl.org/ontology/pbo/core#skip_object">
    <rdfs:comment xml:lang="en">Associates a skip object to its related skip counter.</rdfs:comment>
    <rdfs:isDefinedBy rdf:resource="http://purl.org/ontology/pbo/core#"/>
    <rdfs:label xml:lang="en">has skip object</rdfs:label>
    <rdfs:range>
      <rdf:Description>
        <owl:unionOf>
          <rdf:Description>
            <rdf:first rdf:resource="http://purl.org/ontology/bibo/Document"/>
            <rdf:rest>
              <rdf:Description>
                <rdf:first rdf:resource="http://purl.org/vocab/frbr/core#Endeavour"/>
                <rdf:rest rdf:resource="http://www.w3.org/1999/02/22-rdf-syntax-ns#nil"/>
              </rdf:Description>
            </rdf:rest>
          </rdf:Description>
        </owl:unionOf>
      </rdf:Description>
    </rdfs:range>
    <rdfs:subPropertyOf rdf:resource="http://purl.org/ontology/co/core#object"/>
    <vs:term_status xml:lang="en">unstable</vs:term_status>
  </owl:ObjectProperty>
</rdf:RDF>
